UecInLean/TaPL/Arithmetic.lean
@@ -1,0 +1,123 @@
+import Init.WF
+
+namespace UecInLean.TaPL
+
+class Derivable (T : Type) where
+  derivable : T -> T -> Prop
+infix:100 " ⟶ " => Derivable.derivable
+
+section NormalForm
+
+variable {T : Type} [Derivable T]
+
+def isNormalForm (t : T) := ∀ t', ¬ t ⟶ t'
+
+/-- 定義 3.5.6 -/
+theorem isNormalForm_iff (t : T) : isNormalForm t ↔ ¬ ∃ t', t ⟶ t' := by rw [isNormalForm, not_exists]
+
+theorem isNormalForm_not_iff (t : T) : ¬ isNormalForm t ↔ ∃ t', t ⟶ t' := by simp only [isNormalForm, Classical.not_forall, Classical.not_not]
+
+theorem contra_of_isNormalForm_of_deriv {t t' : T} (h : isNormalForm t) (h' : t ⟶ t') : False := h t' h'
+
+theorem isNormalForm_of_pre {τ : T -> T} (hτ : ∀ {s s'}, s ⟶ s' -> τ s ⟶ τ s') {t : T} (ht : isNormalForm (τ t)) : isNormalForm t := by {
+  intro t' h
+  exact ht (τ t') (hτ h)
+}
+
+end NormalForm
+
+class HasValue (T : Type) where
+  isValue : T -> Prop
+
+section MultiStepDeriv
+
+/-- 定義 3.5.9 -/
+inductive MultiStepDeriv {T : Type} [Derivable T] (t : T) : T -> Prop
+  | refl : MultiStepDeriv t t
+  | step {t' t''} : t'' ⟶ t' -> MultiStepDeriv t t' -> MultiStepDeriv t t''
+notation:100 a:100 " ⟶* " b:100 => MultiStepDeriv b a
+
+variable {T : Type} [Derivable T]
+
+theorem MultiStepDeriv.lift {t t' : T} (h : t ⟶ t') : t ⟶* t' := .step h .refl
+
+instance {t t' : T} : Coe (t ⟶ t') (t ⟶* t') := ⟨MultiStepDeriv.lift⟩
+
+theorem MultiStepDeriv.append {t t' t'' : T} (h : t ⟶* t') (h' : t' ⟶* t'') : t ⟶* t'' := by {
+  induction h with
+  | refl => exact h'
+  | step h hs ih => exact .step h ih
+}
+
+theorem MultiStepDeriv.two {t t' t'' : T} (h : t ⟶ t') (h' : t' ⟶ t'') : t ⟶* t'' := by {
+  exact MultiStepDeriv.append (.lift h) (.lift h')
+}
+
+theorem MultiStepDeriv.inherit {τ : T -> T} (hτ : ∀ {s s'}, s ⟶ s' -> τ s ⟶ τ s') : ∀ {t₁ t₁'}, t₁ ⟶* t₁' -> τ t₁ ⟶* τ t₁' := by {
+  intro _ _ h
+  induction h with
+  | refl => exact .refl
+  | step h _ ih => exact .step (hτ h) ih
+}
+
+end MultiStepDeriv
+
+section Halting
+
+class Halting (T : Type) [Derivable T] where
+  measure : T -> Nat
+  ordering {t t' : T} : t ⟶ t' → measure t' < measure t
+
+variable {T : Type} [Derivable T] [Halting T]
+
+instance : WellFoundedRelation T := measure Halting.measure
+
+/-- 定理 3.5.12 -/
+theorem evaluation_halting (t : T) : ∃ t', isNormalForm t' ∧ t ⟶* t' := by {
+  rcases Classical.em (isNormalForm t) with h | h
+  {
+    exact ⟨t, h, .refl⟩
+  }
+  {
+    rw [isNormalForm_not_iff] at h
+    rcases h with ⟨t', ht⟩
+    have := Halting.ordering ht
+    have ⟨t'', ht'', h''⟩ := evaluation_halting t'
+    exact ⟨t'', ht'', .step ht h''⟩
+  }
+}
+termination_by Halting.measure t
+
+end Halting
+
+section Arithmetic
+
+class Arithmetic (T : Type) extends Derivable T, HasValue T, Halting T where
+  /-- 定理 3.5.4 -/
+  determination {t t' t'' : T} : t ⟶ t' → (t ⟶ t'') → t' = t''
+  /-- 定理 3.5.7 -/
+  isNormalForm_of_isValue (t : T) : isValue t → isNormalForm t
+
+variable {T : Type} [inst : Arithmetic T]
+
+/-- 定理 3.5.11 -/
+theorem NormalForm_unique {t u u' : T} (hu : isNormalForm u) (hu' : isNormalForm u') (h : t ⟶* u) (h' : t ⟶* u') : u = u' := by {
+  induction h with
+  | refl => {
+    cases h' with
+    | refl => rfl
+    | step h' => exact absurd h' (hu _)
+  }
+  | step h hs ih => {
+    cases h' with
+    | refl => exact absurd h (hu' _)
+    | step h' hs' => {
+      rw [← inst.determination h h'] at hs'
+      exact ih hs'
+    }
+  }
+}
+
+end Arithmetic
+
+def isDeadlock {T : Type} [Derivable T] [HasValue T] (t : T) : Prop := isNormalForm t ∧ ¬ HasValue.isValue t
